store/client_proofs/store.v
@@ -5,7 +5,7 @@ From iris.algebra Require Import agree auth csum gset gmap excl frac.
 From iris.algebra Require Import max_prefix_list.
 From iris.heap_lang Require Import notation proofmode.
 From cryptis Require Import lib version term cryptis primitives tactics.
-From cryptis Require Import role dh_auth.
+From cryptis Require Import role iso_dh.
 From cryptis.store Require Import impl shared db connection_proofs.
 
 Set Implicit Arguments.
